stubbing out everything. working on reification issues.

src/sep/Array8.v
@@ -248,10 +248,10 @@ Section correctness.
     rewrite natToW_S.
     rewrite wplus_assoc.
     eapply split_smem_get; eauto.
-    right.
+    (* right.
     apply IHbs; try omega.
-    propxFo.
-  Qed.
+    propxFo. *)
+  Admitted.
 
   Lemma array8_bound' : forall cs base stn bs m i,
     (0 < i < length bs)%nat
@@ -340,6 +340,7 @@ Section correctness.
     rewrite natToWord_wordToNat in H0; auto.
   Qed.
 
+(*
   Lemma sym_read_correct : forall P (PE : ProverT_correct P funcs),
     forall args uvars vars cs facts pe p ve stn st,
       sym_read P facts args pe = Some ve ->
@@ -349,16 +350,16 @@ Section correctness.
         applyD (exprD funcs uvars vars) (SEP.SDomain ssig) args _ (SEP.SDenotation ssig)
         with
         | None => False
-        | Some p => ST.satisfies cs p stn st
+        | Some p => PropX.interp cs (p stn st)
       end ->
-      match ST.HT.smem_get p st with
+      match IL.smem_read p st with
         | Some b => exprD funcs uvars vars ve wordT = Some (BtoW b)
         | _ => False
       end.
   Proof.
     simpl; intuition.
     do 3 (destruct args; simpl in *; intuition; try discriminate).
-    generalize (deref_correct uvars vars pe); destr ltac:(simpl in *) (deref pe); intro Hderef.
+    generalize (deref_correct uvars vars pe); destr ltac:(simpl in * ) (deref pe); intro Hderef.
     destruct p0.
 
     repeat match goal with
@@ -446,6 +447,7 @@ Section correctness.
     auto.
   Qed.
 
+
   Lemma sym_write_correct' : forall i bs p specs stn st v,
     i < natToW (length bs)
     -> interp specs (array8 bs p stn st)
@@ -490,7 +492,7 @@ Section correctness.
   Proof.
     simpl; intuition.
     do 3 (destruct args; simpl in *; intuition; try discriminate).
-    generalize (deref_correct uvars vars pe); destr ltac:(simpl in *) (deref pe); intro Hderef.
+    generalize (deref_correct uvars vars pe); destr ltac:(simpl in * ) (deref pe); intro Hderef.
     destruct p0.
 
     repeat match goal with
@@ -525,11 +527,12 @@ Section correctness.
     destruct H3; intuition.
     rewrite H7; assumption.
   Qed.
+*)
 End correctness.
 
-Definition MemEvaluator types' : MEVAL.MemEvaluator (types types') (tvType 0) (tvType 1) :=
+Definition MemEvaluator types' : MEVAL.MemEvaluator (types types') :=
   Eval cbv beta iota zeta delta [ MEVAL.PredEval.MemEvalPred_to_MemEvaluator ] in 
-    @MEVAL.PredEval.MemEvalPred_to_MemEvaluator _ (tvType 0) (tvType 1) (MemEval types') 3.
+    @MEVAL.PredEval.MemEvalPred_to_MemEvaluator _ (MemEval types') 3.
 
 Theorem MemEvaluator_correct types' funcs' preds'
   : @MEVAL.MemEvaluator_correct (Env.repr types_r types') (tvType 0) (tvType 1) 
@@ -540,10 +543,14 @@ Theorem MemEvaluator_correct types' funcs' preds'
 Proof.
   intros. eapply (@MemPredEval_To_MemEvaluator_correct (types types')); try reflexivity;
   intros; unfold MemEval in *; simpl in *; try discriminate.
+  admit.
+  admit.
+(*
   { generalize (@sym_read_correct types' funcs' P PE). simpl in *. intro.
     eapply H3 in H; eauto. }
   { generalize (@sym_write_correct types' funcs' P PE). simpl in *. intro.
     eapply H4 in H; eauto. }
+*)
 Qed.
 
 Definition pack : MEVAL.MemEvaluatorPackage types_r (tvType 0) (tvType 1) (tvType 0) (tvType 0)
@@ -554,7 +561,6 @@ Definition pack : MEVAL.MemEvaluatorPackage types_r (tvType 0) (tvType 1) (tvTyp
   types_r
   funcs_r
   (fun ts => Env.listOptToRepr (None :: None :: None :: Some (ssig ts) :: nil)
-    (SEP.Default_predicate (Env.repr types_r ts)
-      (tvType 0) (tvType 1)))
+    (SEP.Default_predicate (Env.repr types_r ts)))
   (fun ts => MemEvaluator _)
   (fun ts fs ps => MemEvaluator_correct _ _).
